Lambda_Int_Ext.v
@@ -54,18 +54,20 @@ Inductive ext_lab_contextual_closure (Red : pterm -> pterm -> Prop) : pterm -> p
 Inductive lab_x_i: pterm -> pterm -> Prop :=
 | xi_from_bx_in_les: forall t1 t2 t2', 
                        lab_term (t1 [[ t2 ]]) ->
-                       (t2 -->lex t2') ->
+                       (sys_Bx t2 t2') ->
                        lab_x_i (t1 [[ t2 ]]) (t1 [[ t2' ]])
 | xi_from_x : forall t t', 
                 lab_term t ->
                 lab_sys_x t t' -> 
                 lab_x_i t t'. 
 
-Definition lab_x_i_eq (t: pterm) (u : pterm) := 
-    exists t' u', (t =EE t')/\(ext_lab_contextual_closure lab_x_i t' u')/\(u' =EE u).
+Definition lab_EE_ctx_red (R: pterm -> pterm -> Prop) (t: pterm) (u : pterm) := 
+    exists t' u', (t =EE t')/\(ext_lab_contextual_closure R t' u')/\(u' =EE u).
 
-Definition lab_x_e_eq (t: pterm) (u : pterm) := 
-    exists t' u', (t =EE t')/\((ext_lab_contextual_closure sys_Bx) t' u')/\(u' =EE u).
+
+Definition lab_x_i_eq := lab_EE_ctx_red lab_x_i.
+
+Definition lab_x_e_eq := lab_EE_ctx_red sys_Bx.
 
 Notation "t -->[lx_i] u" := (lab_x_i_eq t u) (at level 59, left associativity).
 Notation "t -->[lx_e] u" := (lab_x_e_eq t u) (at level 59, left associativity).
@@ -78,16 +80,6 @@ Proof.
     constructor 2. exists t u. split*. split. constructor 1. constructor 2. auto. auto. 
     constructor 1. exists t u. split*. split. constructor 1. auto. constructor 2. auto. auto. auto.
 Qed.
-
-(*Lemma lab_x_i_sys_lx: forall t t', lab_x_i t t' -> lab_sys_lx t t'.*)
-(*Proof.*)
-    (*intros.*)
-    (*induction H.*)
-    (*destruct H0.  destruct H0.*)
-    (*destruct H0.*)
-    (*destruct H1.*)
-    (*induction H1.*)
-(*Qed.*)
 
 Lemma eqcc_lab_term: forall t t', lab_term t -> t =ee t' -> lab_term t'.
 Proof.
@@ -156,7 +148,45 @@ Proof.
     constructor 2 with (pterm_app u u0); auto.
 Qed.
 
+Lemma EE_clos_app_left: forall R t t' u, lab_term u -> ((lab_EE_ctx_red R) t t') -> ((lab_EE_ctx_red R) (pterm_app t u) (pterm_app t' u)).
+Proof.
+    intros.
+    destruct H0.
+    destruct H0.
+    destruct H0.
+    destruct H1.
+    exists (pterm_app x u) (pterm_app x0 u).
+    split. apply star_lab_closure_app_left; auto.
+    split*. constructor 2; auto.
+    apply star_lab_closure_app_left; auto.
+
+Qed.
+
+Lemma EE_clos_app_right: forall R t t' u, lab_term u -> ((lab_EE_ctx_red R) t t') -> ((lab_EE_ctx_red R) (pterm_app u t) (pterm_app u t')).
+Proof.
+    intros.
+    destruct H0.
+    destruct H0.
+    destruct H0.
+    destruct H1.
+    exists (pterm_app u x) (pterm_app u x0).
+    split. apply star_lab_closure_app_right; auto.
+    split*. constructor 3; auto.
+    apply star_lab_closure_app_right; auto.
+
+Qed.
+
+
+
 Lemma pterm_abs_EE_inversion: forall t v, (pterm_abs t) =EE v -> exists t', v = (pterm_abs t') /\ (t =EE t').
+Proof.
+    Admitted.
+
+Lemma red_rename_lab_xi_eq: red_rename lab_x_i_eq.
+Proof.
+    Admitted.
+
+Lemma red_rename_lab_xe_eq: red_rename lab_x_e_eq.
 Proof.
     Admitted.
 
@@ -164,9 +194,51 @@ Lemma lx_i_open_abs: forall x x0 L, (forall y : VarSet.elt, y \notin L -> x0 ^ y
 Proof.
     Admitted.
 
+Lemma lx_e_open_abs: forall x x0 L, (forall y : VarSet.elt, y \notin L -> x0 ^ y-->[lx_e]x ^ y) -> pterm_abs x0-->[lx_e]pterm_abs x.
+Proof.
+    Admitted.
+
 Lemma term_EE_open: forall t t' x, t =EE t' -> (t ^ x) =EE (t' ^ x).
 Proof.
     Admitted.
+
+Lemma EE_lab_term : forall t t', lab_term t -> t =EE t' -> lab_term t'.
+Proof.
+    Admitted.
+
+Lemma lab_sys_lx_term_is_sys_Bx : forall t t', term t -> lab_sys_lx t t' -> sys_Bx t t'.
+Proof.
+    Admitted.
+
+
+Lemma pterm_sub_EE_inversion: forall t u v, (t[u]) =EE v -> (exists t', v = (t'[u])) \/ (exists t' u', v = (t'[u'])) \/ (exists t' u', v = (t'[[u']])).
+Proof.
+    Admitted.
+
+
+Lemma EE_presv_ie: forall t t' u u', t =EE u -> u' =EE t' -> ((u -->[lx_i] u' \/ u -->[lx_e] u') -> (t -->[lx_i] t' \/ t -->[lx_e] t')).
+Proof.
+    intros.
+
+    destruct H1.  destruct H1.  destruct H1.  destruct H1. destruct H2.
+    left.  
+    exists x x0.
+    split*.
+    (*apply star_ctx_eqcc_sym in H.*)
+    apply star_closure_composition with u; auto.
+    split*.
+    apply star_closure_composition with u'; auto.
+
+    destruct H1.  destruct H1.  destruct H1.  destruct H2.
+    right.  
+    exists x x0.
+    split*.
+    apply star_ctx_eqcc_sym in H.
+    apply star_ctx_eqcc_sym in H.
+    apply star_closure_composition with u; auto.
+    split*.
+    apply star_closure_composition with u'; auto.
+Qed.
 
 Lemma lab_ex_eq_i_e: forall t t', lab_term t -> (t -->[lex] t' <-> (t -->[lx_i] t' \/ t -->[lx_e] t')).
 Proof.
@@ -180,103 +252,209 @@ Proof.
     (* Base *)
     apply lab_sys_x_i_e with t s; auto. apply star_ctx_eqcc_lab_term with t0; auto*.
 
-    (* app left *)
-    assert (H4 := pterm_app_EE_inversion H2).
-    apply star_ctx_eqcc_sym in H3.
-    assert (H5 := pterm_app_EE_inversion H3).
-    destruct H4.  destruct H4.  destruct H4.  destruct H6.  
-    destruct H5.  destruct H5.  destruct H5.  destruct H8.
-    subst. inversion H0; subst.  apply star_ctx_eqcc_sym in H8.
-    assert (x1-->[lx_i]x \/ x1-->[lx_e]x).  apply IHlab_contextual_closure; auto.
-    destruct H4. left. 
-    destruct H4. destruct H4. destruct H4. destruct H5.
-    exists (pterm_app x3 u) (pterm_app x4 u).
-    split. apply star_closure_composition with (pterm_app x1 u).
-    apply star_lab_closure_app_right. auto. apply star_ctx_eqcc_sym in H9. auto.
-    apply star_lab_closure_app_left. auto. auto.
-    split. constructor 2; auto. apply star_closure_composition with (pterm_app x u).
-    apply star_lab_closure_app_left; auto. apply star_lab_closure_app_right; auto.
-    admit.
-    right.
-    destruct H4. destruct H4. destruct H4. destruct H5.
-    exists (pterm_app x3 u) (pterm_app x4 u).
-    split. apply star_closure_composition with (pterm_app x1 u).
-    apply star_lab_closure_app_right. auto. apply star_ctx_eqcc_sym in H9. auto.
-    apply star_lab_closure_app_left. auto. auto.
-    split. constructor 2; auto. apply star_closure_composition with (pterm_app x u).
-    apply star_lab_closure_app_left; auto. apply star_lab_closure_app_right; auto.
-    admit.
+    (* app_left *)
 
-    (* app right *)
-    assert (H4 := pterm_app_EE_inversion H2).
-    apply star_ctx_eqcc_sym in H3.
-    assert (H5 := pterm_app_EE_inversion H3).
-    destruct H4.  destruct H4.  destruct H4.  destruct H6.  
-    destruct H5.  destruct H5.  destruct H5.  destruct H8.
-    subst. inversion H0; subst.  apply star_ctx_eqcc_sym in H9.
-    assert (x2-->[lx_i]x0 \/ x2-->[lx_e]x0).  apply IHlab_contextual_closure; auto.
-    destruct H4. left. 
-    destruct H4. destruct H4. destruct H4. destruct H5.
-    exists (pterm_app t x3) (pterm_app t x4).
-    split. apply star_closure_composition with (pterm_app x1 x3).
-    apply star_lab_closure_app_right. auto.  auto.
-    apply star_lab_closure_app_left. admit. apply star_ctx_eqcc_sym in H8. auto. 
-    split. constructor 3; auto. apply star_closure_composition with (pterm_app x x4).
-    apply star_lab_closure_app_left; auto. admit. apply star_lab_closure_app_right; auto.
-    admit.
-    right.
-    destruct H4. destruct H4. destruct H4. destruct H5.
-    exists (pterm_app t x3) (pterm_app t x4).
-    split. apply star_closure_composition with (pterm_app x1 x3).
-    apply star_lab_closure_app_right. auto.  auto.
-    apply star_lab_closure_app_left. admit. apply star_ctx_eqcc_sym in H8. auto. 
-    split. constructor 3; auto. apply star_closure_composition with (pterm_app x x4).
-    apply star_lab_closure_app_left; auto. admit. apply star_lab_closure_app_right; auto.
-    admit.
+    (*apply star_ctx_eqcc_sym in H3.*)
+    apply EE_presv_ie with (u := (pterm_app t u)) (u' := (pterm_app t' u)); auto.
+    assert  (t-->[lx_i]t' \/ t-->[lx_e]t').
+    apply IHlab_contextual_closure; auto. constructor 1; auto. admit. constructor 1; auto.
+    destruct H4. 
+    left. apply EE_clos_app_left. admit. auto.
+    right. apply EE_clos_app_left. admit. auto.
+
+
+    (* app_right *)
+    (*apply star_ctx_eqcc_sym in H3.*)
+    apply EE_presv_ie with (u := (pterm_app t u)) (u' := (pterm_app t u')); auto.
+    assert  (u-->[lx_i]u' \/ u-->[lx_e]u').
+    apply IHlab_contextual_closure; auto. constructor 1; auto. admit. constructor 1; auto.
+    destruct H4. 
+    left. apply EE_clos_app_right. admit. auto.
+    right. apply EE_clos_app_right. admit. auto.
 
     (* abs *)
-    assert (H4 := pterm_abs_EE_inversion H2).
-    apply star_ctx_eqcc_sym in H3.
-    assert (H5 := pterm_abs_EE_inversion H3).
-    destruct H4.  destruct H4. 
-    destruct H5.  destruct H5. 
-    subst. inversion H1; subst. 
-    (*assert (forall y, y \notin (L \u L0) -> x0 ^ y -->[lx_i] x ^ y ).*)
-    (*intros.*)
-    (*apply term_EE_open with t' x y in H6.*)
-    (*apply term_EE_open with t x0 y in H7.*)
-    (*apply notin_union in H4. destruct H4.*)
-    (*pose proof (H5 y H8); auto.*)
-    (*apply star_ctx_eqcc_sym in H7.*)
-    (*pose proof (H0 y H4 (x ^ y) H6 (x0 ^ y) H9 H7). admit.*)
-    (*left. *)
-    assert (forall y, y \notin (L \u L0) -> x0 ^ y -->[lx_i] x ^ y \/  x0 ^ y -->[lx_e] x ^ y ).
-    intros.
-    apply term_EE_open with t' x y in H6.
-    apply term_EE_open with t x0 y in H7.
-    apply notin_union in H4. destruct H4.
-    pose proof (H5 y H8); auto.
-    apply star_ctx_eqcc_sym in H7.
-    pose proof (H0 y H4 (x ^ y) H6 (x0 ^ y) H9 H7). auto.
-    (*assert ((forall y : VarSet.elt, y \notin L \u L0 -> x0 ^ y-->[lx_i]x ^ y) \/ (forall y : VarSet.elt, y \notin L \u L0 -> x0 ^ y-->[lx_e]x ^ y)). admit.*)
-    (*destruct H8. left. apply lx_i_open_abs with (L \u L0). auto.*)
-    (*exists (pterm_abs x0) (pterm_abs x). *)
-    (*split. constructor 1. split. constructor 4 with (L \u L0). intros. *)
-    (*pose proof ( H8 x1 H9 ). destruct H10. destruct H10.*)
-
-
-    (*inversion H2; subst. inversion H4; subst. inversion H4; subst.*)
-    (*inversion H2; subst. inversion H4; subst. inversion H4; subst.*)
-    (*inversion H2; subst. inversion H4; subst. inversion H4; subst.*)
-    (*inversion H2; subst. inversion H5; subst.*)
-
-    (*Focus 7.*)
-    (*intros. destruct H0; destruct H0; destruct H0; destruct H0; destruct H1; induction H1.*)
-    (*exists t0 s. split*. split*. constructor 1; auto. constructor.*)
-    (*exists (t1 [[t2]]) (t1 [[t2']]). split*. split. constructor 8. inversion H1. *)
-    (*exists L; auto. inversion H1; auto.  inversion H3. constructor 1; auto.*)
-    (*constructor 2; auto. auto. *)
-
-
+    apply EE_presv_ie with (u := pterm_abs t) (u' := pterm_abs t'); auto.
+    pick_fresh z.
+    assert  (t^z-->[lx_i]t'^z \/ t^z-->[lx_e]t'^z).
+    apply H0 with z; auto. constructor 1; auto. admit. constructor 1; auto. 
+    apply notin_union in Fr; destruct Fr.
+    apply notin_union in H5; destruct H5.
+    apply notin_union in H5; destruct H5.
+    apply notin_union in H5; destruct H5.
 
 Qed.
+
+(*Lemma lab_ex_eq_i_e: forall t t', lab_term t -> (t -->[lex] t' <-> (t -->[lx_i] t' \/ t -->[lx_e] t')).*)
+(*Proof.*)
+    (*split.*)
+    (*intro.*)
+    (*destruct H0.  destruct H0. destruct H0.  destruct H1.*)
+    (*generalize dependent t.*)
+    (*generalize dependent t'.*)
+    (*induction H1; intros.*)
+
+    (*[> Base <]*)
+    (*apply lab_sys_x_i_e with t s; auto. apply star_ctx_eqcc_lab_term with t0; auto*.*)
+
+    (*[> app left <]*)
+    (*assert (H4 := pterm_app_EE_inversion H2).*)
+    (*apply star_ctx_eqcc_sym in H3.*)
+    (*assert (H5 := pterm_app_EE_inversion H3).*)
+    (*destruct H4.  destruct H4.  destruct H4.  destruct H6.  *)
+    (*destruct H5.  destruct H5.  destruct H5.  destruct H8.*)
+    (*subst. inversion H0; subst.  apply star_ctx_eqcc_sym in H8.*)
+    (*assert (x1-->[lx_i]x \/ x1-->[lx_e]x).  apply IHlab_contextual_closure; auto.*)
+    (*destruct H4. left. *)
+    (*destruct H4. destruct H4. destruct H4. destruct H5.*)
+    (*exists (pterm_app x3 u) (pterm_app x4 u).*)
+    (*split. apply star_closure_composition with (pterm_app x1 u).*)
+    (*apply star_lab_closure_app_right. auto. apply star_ctx_eqcc_sym in H9. auto.*)
+    (*apply star_lab_closure_app_left. auto. auto.*)
+    (*split. constructor 2; auto. apply star_closure_composition with (pterm_app x u).*)
+    (*apply star_lab_closure_app_left; auto. apply star_lab_closure_app_right; auto.*)
+    (*admit.*)
+    (*right.*)
+    (*destruct H4. destruct H4. destruct H4. destruct H5.*)
+    (*exists (pterm_app x3 u) (pterm_app x4 u).*)
+    (*split. apply star_closure_composition with (pterm_app x1 u).*)
+    (*apply star_lab_closure_app_right. auto. apply star_ctx_eqcc_sym in H9. auto.*)
+    (*apply star_lab_closure_app_left. auto. auto.*)
+    (*split. constructor 2; auto. apply star_closure_composition with (pterm_app x u).*)
+    (*apply star_lab_closure_app_left; auto. apply star_lab_closure_app_right; auto.*)
+    (*admit.*)
+
+    (*[> app right <]*)
+    (*assert (H4 := pterm_app_EE_inversion H2).*)
+    (*apply star_ctx_eqcc_sym in H3.*)
+    (*assert (H5 := pterm_app_EE_inversion H3).*)
+    (*destruct H4.  destruct H4.  destruct H4.  destruct H6.  *)
+    (*destruct H5.  destruct H5.  destruct H5.  destruct H8.*)
+    (*subst. inversion H0; subst.  apply star_ctx_eqcc_sym in H9.*)
+    (*assert (x2-->[lx_i]x0 \/ x2-->[lx_e]x0).  apply IHlab_contextual_closure; auto.*)
+    (*destruct H4. left. *)
+    (*destruct H4. destruct H4. destruct H4. destruct H5.*)
+    (*exists (pterm_app t x3) (pterm_app t x4).*)
+    (*split. apply star_closure_composition with (pterm_app x1 x3).*)
+    (*apply star_lab_closure_app_right. auto.  auto.*)
+    (*apply star_lab_closure_app_left. admit. apply star_ctx_eqcc_sym in H8. auto. *)
+    (*split. constructor 3; auto. apply star_closure_composition with (pterm_app x x4).*)
+    (*apply star_lab_closure_app_left; auto. admit. apply star_lab_closure_app_right; auto.*)
+    (*admit.*)
+    (*right.*)
+    (*destruct H4. destruct H4. destruct H4. destruct H5.*)
+    (*exists (pterm_app t x3) (pterm_app t x4).*)
+    (*split. apply star_closure_composition with (pterm_app x1 x3).*)
+    (*apply star_lab_closure_app_right. auto.  auto.*)
+    (*apply star_lab_closure_app_left. admit. apply star_ctx_eqcc_sym in H8. auto. *)
+    (*split. constructor 3; auto. apply star_closure_composition with (pterm_app x x4).*)
+    (*apply star_lab_closure_app_left; auto. admit. apply star_lab_closure_app_right; auto.*)
+    (*admit.*)
+
+    (*[> abs <]*)
+    (*assert (H4 := pterm_abs_EE_inversion H2).*)
+    (*apply star_ctx_eqcc_sym in H3.*)
+    (*assert (H5 := pterm_abs_EE_inversion H3).*)
+    (*destruct H4.  destruct H4. *)
+    (*destruct H5.  destruct H5. *)
+    (*subst. inversion H1; subst. *)
+
+    (*assert ((forall y, y \notin (L \u L0) -> x0 ^ y -->[lx_i] x ^ y) \/  (forall y, y \notin (L \u L0) -> x0 ^ y -->[lx_e] x ^ y )).*)
+    (*pick_fresh z.*)
+    (*apply term_EE_open with t' x z in H6.*)
+    (*apply term_EE_open with t x0 z in H7.*)
+    (*apply notin_union in Fr. destruct Fr.  apply notin_union in H4. destruct H4.  *)
+    (*apply notin_union in H4. destruct H4.  apply notin_union in H4. destruct H4.  *)
+    (*apply notin_union in H4. destruct H4.  *)
+    (*pose proof (H5 z H12); auto.*)
+    (*apply star_ctx_eqcc_sym in H7.*)
+    (*pose proof (H0 z H4 (x ^ z) H6 (x0 ^ z) H13 H7). *)
+    (*clear H11 H10. auto.*)
+    (*destruct H14.*)
+    (*left. intros.*)
+    (*pose proof red_rename_lab_xi_eq.*)
+    (*apply H14 with z; auto.*)
+    (*right; intros.*)
+    (*pose proof red_rename_lab_xe_eq.*)
+    (*apply H14 with z; auto.*)
+    (*destruct H4. *)
+    (*left. apply lx_i_open_abs with (L \u L0); auto.*)
+    (*right. apply lx_e_open_abs with (L \u L0); auto.*)
+
+    (*[> sub <]*)
+
+    (*pose proof H2. apply pterm_sub_EE_inversion in H2. *)
+    (*pose proof H4. apply star_ctx_eqcc_sym in H4. apply pterm_sub_EE_inversion in H4. *)
+    (*destruct H2. destruct H2; subst. *)
+    (*destruct H4. destruct H2; subst.*)
+    (*admit.*)
+    (*destruct H2. destruct H2; subst. destruct H2; subst.*)
+
+
+    (*[>fail.<]*)
+    (*Focus 6. [> u --> u' <]*)
+    (*[>inversion H2; subst.<]*)
+    (*[>inversion H3; subst.<]*)
+    (*left. exists (t [[u]]) (t [[u']]). split. auto.*)
+    (*split*. *)
+    (*apply EE_lab_term in H3.*)
+    (*inversion H3; subst.*)
+    (*apply lab_sys_lx_term_is_sys_Bx in H0; auto.*)
+    (*inversion H0; subst.*)
+    (*constructor 1.  constructor 1. auto. auto.*)
+    (*constructor 1.  constructor 1. auto. constructor 2; auto. *)
+    (*auto.*)
+    (*[>constructor 6. constructor 2. auto. admit. constructor 2; auto. <]*)
+    (*[>constructor 1; auto. constructor 2; auto. admit. [> !!! <]<]*)
+    (*[>inversion H2; subst. inversion H4; subst. inversion H4; subst.<]*)
+    (*[>inversion H2; subst. inversion H4; subst. inversion H4; subst.<]*)
+    (*[>inversion H2; subst. inversion H4; subst. inversion H4; subst.<]*)
+    (*[>inversion H2; subst. inversion H5; subst.<]*)
+
+    (*Focus 4.*)
+    (*[> i_e -> ex <]*)
+    (*intros. destruct H0; destruct H0; destruct H0; destruct H0; destruct H1; generalize dependent t; generalize dependent t'; induction H1; intros.*)
+
+    (*[> Interna <]*)
+    (*[> Base <]*)
+    (*inversion H; subst. *)
+    (*exists (t1 [[t2]]) (t1 [[t2']]). *)
+    (*split*. split*. *)
+    (*constructor 8. admit. inversion H4; subst.*)
+    (*constructor 1; auto.  constructor 2; subst. auto. *)
+    (*exists t s. split*. constructor 1; auto. constructor 1. constructor 3; auto.*)
+
+    (*[> app_l <]*)
+    (*assert (H4 := pterm_app_EE_inversion H2).*)
+    (*apply star_ctx_eqcc_sym in H3.*)
+    (*assert (H5 := pterm_app_EE_inversion H3).*)
+    (*destruct H4.  destruct H4.  destruct H4.  destruct H6.  *)
+    (*destruct H5.  destruct H5.  destruct H5.  destruct H8.*)
+    (*subst. inversion H0; subst.  apply star_ctx_eqcc_sym in H8.*)
+    (*assert ( x1-->[lex]x ). apply IHext_lab_contextual_closure; auto. *)
+    (*destruct H4.  destruct H4.  destruct H4.  destruct H5.*)
+    (*exists (pterm_app x3 u) (pterm_app x4 u). split*. *)
+    (*apply star_closure_composition with (pterm_app x1 u).*)
+    (*apply star_lab_closure_app_right; auto. apply star_ctx_eqcc_sym; auto.*)
+    (*apply star_lab_closure_app_left; auto. split*. constructor 2; auto.*)
+    (*apply star_closure_composition with (pterm_app x u). *)
+    (*apply star_lab_closure_app_left; auto. apply star_lab_closure_app_right; auto.*)
+    (*admit.*)
+
+    (*[> app_r <]*)
+    (*assert (H4 := pterm_app_EE_inversion H2).*)
+    (*apply star_ctx_eqcc_sym in H3.*)
+    (*assert (H5 := pterm_app_EE_inversion H3).*)
+    (*destruct H4.  destruct H4.  destruct H4.  destruct H6.  *)
+    (*destruct H5.  destruct H5.  destruct H5.  destruct H8.*)
+    (*subst. inversion H0; subst.  apply star_ctx_eqcc_sym in H9.*)
+    (*assert ( x2-->[lex]x0 ). apply IHext_lab_contextual_closure; auto. *)
+    (*destruct H4.  destruct H4.  destruct H4.  destruct H5.*)
+    (*exists (pterm_app t x3) (pterm_app t x4). split*. *)
+    (*apply star_closure_composition with (pterm_app t x2).*)
+    (*apply star_lab_closure_app_left; auto. apply star_ctx_eqcc_sym; auto.*)
+    (*apply star_lab_closure_app_right; auto. split*. constructor 3; auto.*)
+    (*apply star_closure_composition with (pterm_app x x4). *)
+    (*apply star_lab_closure_app_left; auto. admit. apply star_lab_closure_app_right; auto.*)
+    (*admit.*)
+
+(*Qed.*)
